\chapter{Basic Principles}

\section{The Laplace Transform}

\begin{exercise}
\item
  From the definition of the Laplace transform compute
  \(\mathcal{L}\{f(t)\}(s)\)
  for
  \begin{exercise}[label = (\alph*), ref = \arabic{exercisei} (\alph*)]
  \item
    \(f(t) = 4t\)
    \par\smallskip
    The Laplace transform is defined as
    \(\mathcal{L}\{f(t)\}(s) = \int_0^{\infty}f(t)e^{-st}dt\).
    Using the definition, we have
    \[
    \mathcal{L}\{4t\}(s) = \int_0^{\infty}4te^{-st}dt =
    4\lim_{\tau\to\infty}\int_0^{\tau}te^{-st}dt
    \]
    We can now use integration by parts or we may notice that
    \(-\frac{\partial}{\partial s}e^{-st} = te^{-st}\).
    Note that \(t\) and \(e^{-st}\) are entire functions in both the variable
    \(s\) and \(t\); that is, \(t\) and \(e^{-st}\) can be represented by a
    power series that converges everywhere in the complex plane with an
    infinite radius of convergence.
    In order to justify differentiation under the integral sign, the following
    theorem must be satisfied.
    \par\smallskip
    \textbf{Theorem:} Let \(f(s,t)\) be a function such that both \(f(s,t)\)
    and its partial derivatives are continuous in \(s\) and \(t\) in some
    region of the \((s,t)\)-plane, including \(a(s)\leq t\leq b(s)\),
    \(s_0\leq s\leq s_1\).
    Also suppose that the functions \(a(s)\) and \(b(s)\) are both continuous
    and both have continuous derivatives for \(s_0\leq s\leq s_1\).
    Then for \(s_0\leq s\leq s_1\)
    \[
    \frac{d}{ds}\int_{a(s)}^{b(s)}f(s, t)dt = f(s, b(s))b'(s) - f(s,(a(s))a'(s)
    + \int_{a(s)}^{b(s)}f_s(s, t)dt.
    \]
    Since \(f(s,t) = te^{-st}\) which is the product of two entire functions
    so is entire and \(t,e^{-st}\in C^{\infty}\), the theorem is satisfied.
    Therefore, we can write
    \begin{align*}
      4\lim_{\tau\to\infty}\int_0^{\tau}te^{-st}dt
      & = -4\frac{d}{ds}\lim_{\tau\to\infty}\int_0^{\tau}e^{-st}dt\\
      & = 4\frac{d}{ds}\lim_{\tau\to\infty}\frac{e^{-st}}{s}\Bigr|_0^{\tau}\\
      & = 4\frac{d}{ds}\lim_{\tau\to\infty}
        \Bigl(\frac{e^{-s\tau} - 1}{s}\Bigr)\\
      & = \frac{d}{ds}\frac{-4}{s}\\
      \mathcal{L}\{4t\}(s) & = \frac{4}{s^2}
    \end{align*}
  \item
    \(f(t) = e^{2t}\)
    \par\smallskip
    For brevity, I am going to drop \(\lim_{\tau\to\infty}\int_0^{\tau}\) and
    just write \(\int_0^{\infty}\).
    \[
    \mathcal{L}\{e^{2t}\}(s) = \int_0^{\infty}e^{t(2 - s)}dt =
    \frac{e^{t(2 - s)}}{2 - s}\biggr|_0^{\infty} = \frac{1}{s - 2}
    \]
    A justifiable question would be why don't we have \(\infty\) since
    \(\lim_{t\to\infty}e^{t(2 - s)} = \infty\).
    If this was the case, we would have a divergent integral.
    In order for our integral to converge, we have to mind the exponential
    term.
    Let \(s = \sigma + i\omega\).
    Then \(\exp[2t - \sigma]\exp[-i\omega]\).
    \[
    \biggl\lvert\int_0^{\infty}\exp[(2 - \sigma)t]\exp[-it\omega]dt\biggr\rvert
    \leq\int_0^{\infty}\bigl\lvert\exp[(2 - \sigma)t]\bigr\rvert
    \bigl\lvert\exp[-it\omega]\bigr\rvert dt
    \]
    By Euler's formula, \(\exp[-it\omega] = \cos(t\omega) - i\sin(t\omega)\) so
    \(\lvert e^{-i\omega}\rvert =
    \sqrt{\cos^2(t\omega) + \sin^2(t\omega)} = 1\).
    Thus, we have
    \[
    \int_0^{\infty}\exp[t(2 - \sigma)]dt
    \]
    which converges when \(t(2 - \sigma) < 0\iff 2 < \sigma = \Re\{s\}\).
    Therefore, since \(t(2 - \sigma) < 0\), we are justified in writing
    \(-t(\sigma - 2)\) since \(\sigma - 2 > 0\).
    We then have \(\mathcal{L}\{e^{2t}\}(s) = \frac{1}{s - 2}\).
  \item
    \label{ch1sec1prob1c}
    \(f(t) = 2\cos(3t)\)
    \par\smallskip
    For this problem, we will need to use integration by parts twice.
    Let \(u = e^{-st}\) and \(dv = \cos(3t)dt\).
    Then \(du = -se^{-st}\) and \(v = \sin(3t)/3\)
    \begin{align*}
      \mathcal{L}\{2\cos(3t)\}(s)
      & = 2\int_0^{\infty}\cos(3t)e^{-st}dt\\
      & = \canceltoSwNe{\[\frac{2e^{-st}\sin(3t)}
        {3}\biggl|_0^{\infty}\]}{\(0\)} +
        \frac{2s}{3}\int_0^{\infty}\sin(3t)e^{-st}dt\\
      \intertext{For the second integration by parts, \(u\) and \(du\) will
      remain the same but \(dv = \sin(3t)dt\) so \(v = -\cos(3t)/3\).}
      & = \frac{2s}{3}\Biggl[\frac{-e^{-st}\cos(3t)}{3}\biggl|_0^{\infty} -
        \frac{s}{3}\int_0^{\infty}\cos(3t)e^{-st}dt\Biggr]\\
      (1 + s^2/9)2\int_0^{\infty}\cos(3t)e^{-st}dt & = \frac{2s}{9}\\
      \mathcal{L}\{2\cos(3t)\}(s) & = \frac{2s}{s^2 + 9}
    \end{align*}
  \item
    \(f(t) = 1 - \cos(\omega t)\)
    \par\smallskip
    By \cref{ch1sec1prob1c}, we have
    \[
    \mathcal{L}\{1 - \cos(\omega t)\}(s) = \int_0^{\infty}e^{-st}dt -
    \int_0^{\infty}\cos(\omega t)e^{-st}dt =
    \frac{1}{s} - \frac{s}{s^2 + \omega^2}
    \]
  \item
    \(f(t) = te^{2t}\)
    \[
    \mathcal{L}\{te^{2t}\} = -\frac{\partial }{\partial s}
    \int_0^{\infty}e^{t(2 - s)}dt = -\frac{d}{ds}\frac{1}{s - 2} =
    \frac{1}{(s - 2)^2}
    \]
    where we require that \(\Re\{s\} > 2\).
  \item
    \(f(t) = e^t\sin(t)\)
    \par\smallskip
    Again, we will use integration by parts where \(u = \sin(t)\) and
    \(dv = e^{t(1 - s)}dt\).
    \begin{align*}
      \mathcal{L}\{e^t\sin(t)\}
      & = \int_0^{\infty}\sin(t)e^{t(1 - s)}dt\\
      & = \canceltoSwNe{\[\frac{\sin(t)e^{t(1 - s)}}
        {1 - s}\biggr|_0^{\infty}\]}{\(0\)} +
        \frac{1}{s - 1}\int_0^{\infty}\cos(t)e^{t(1 - s)}dt\\
      & = \frac{1}{s - 1}\Biggl[
        \frac{\cos(t)e^{t(1 - s)}}{1 - s}\biggr|_0^{\infty} - \frac{1}{s - 1}
        \int_0^{\infty}\sin(t)e^{t(1 - s)}dt\Biggr]\\
      [1 + 1/(s + 1)^2]\int_0^{\infty}\sin(t)e^{t(1 - s)}dt
      & = \frac{1}{(s - 1)^2}\\
      \int_0^{\infty}\sin(t)e^{t(1 - s)}dt & = \frac{1}{(s - 1)^2 + 1}
    \end{align*}
  \item
    \(f(t) =
    \begin{cases}
      1, & t\geq a\\
      0, & t < a
    \end{cases}\)
    \begin{align*}
      \mathcal{L}\{f(t)\}(s) & = \int_0^a0\cdot e^{-st}dt +
                               \int_a^{\infty}e^{-st}dt\\
                             & = \int_a^{\infty}e^{-st}dt\\
                             & = \frac{e^{-as}}{s}
    \end{align*}
  \item
    \(f(t) =
    \begin{cases}
      \sin(\omega t), & 0 < t < \pi/\omega\\
      0, & \pi/\omega\leq t
    \end{cases}\)
    \par\smallskip
    This is just another exercise in integration by parts.
    \begin{align*}
      \mathcal{L}\{f(t)\}(s) & = \int_0^{\pi/\omega}\sin(t\omega)e^{-st}dt\\
                             & = \frac{\omega(1 + e^{-s\pi/\omega})}
                               {s^2 + \omega^2}
    \end{align*}
  \item
    \(f(t) =
    \begin{cases}
      2, & t\leq 1\\
      e^t, & t > 1
    \end{cases}\)
    \begin{align*}
      \mathcal{L}\{f(t)\}(s) & = \int_0^1e^{-st}dt +
                               \int_1^{\infty}e^{t(1 - s)}dt\\
                             & = \frac{2(1 - e^{-s})}{s} +
                               \frac{e^{1 - s}}{s - 1}
    \end{align*}
    where we require that \(\Re\{s\} > 1\).
  \end{exercise}
\item
  Compute the Laplace transform of the function \(f(t)\) whose graph is given
  in \cref{ch1sec1}.
  \begin{figure}[H]
    \centering
    \subcaptionbox{\label{ch1sec1prob2a}}{
      \includestandalone[width = 2in, mode = image]{Tikz/ch1sec1prob2a}}
    \qquad
    \subcaptionbox{\label{ch1sec1prob2b}}{
      \includestandalone[width = 3in, mode = image]{Tikz/ch1sec1prob2b}}
    \caption{Plots of \(f(t)\) for problem two.}
    \label{ch1sec1}
  \end{figure}
  The first step to these two problems is to determine the the function
  \(f(t)\).
  For \cref{ch1sec1prob2a}, we have
  \[
  f(t) =
  \begin{cases}
    1 - t, & 0 < t < 1\\
    0, & t > 1
  \end{cases}
  \]
  and for \cref{ch1sec1prob2b}, we have
  \[
  g(t) =
  \begin{cases}
    t, & 0 < t < 1\\
    2 - t, & 1 < t < 2\\
    0, & t > 2
  \end{cases}
  \]
  For \cref{ch1sec1prob2a}, the Laplace transform is
  \begin{align*}
    \mathcal{L}\{f(t)\}(s) & = \int_0^1(1 - t)e^{-st}dt\\
                           & = \frac{1 - e^{-s}}{s} +
                             \frac{\partial }{\partial s}\int_0^1e^{-st}dt\\
                           & = \frac{1 - e^{-s}}{s} + \frac{d}{ds}
                             \frac{1 - e^{-s}}{s}\\
                           & = \frac{s - 1 + e^{-s}}{s^2}
  \end{align*}
  For \cref{ch1sec1prob2b}, the Laplace transform is
  \begin{align*}
    \mathcal{L}\{g(t)\}(s) & = \int_0^1te^{-st}dt + \int_1^2(2 - t)e^{-st}dt\\
                           & = \frac{e^{-2s}(e^s - 1)^2}{s^2}
  \end{align*}
\end{exercise}

\section{Convergence}

\begin{exercise}
\item
  Suppose that \(f\) is a continuous function on \([0,\infty)\) and
  \(\lvert f(t)\rvert\leq M < \infty\) for \(0\leq t < \infty\).
  \begin{exercise}[label = (\alph*), ref = \arabic{exercisei} (\alph*)]
  \item
    Show that the Laplace transform \(F(s) = \mathcal{L}\{f(t)\}(s)\) converges
    absolutely (and hence converges) for any \(s\) satisfying \(\Re\{s\} > 0\).
    \begin{align*}
      \mathcal{L}\{f(t)\}(s) & = \int_0^{\infty}f(t)e^{-st}dt\eqnumtag
                               \label{ch1sec2prob1aLT}\\
      \intertext{In order for the Laplace transform to converge absolutely,
      we need to show that
      \(\lvert\int_0^{\infty}f(t)e^{-st}dt\rvert < \infty\).}
                             & = \biggl\lvert\int_0^{\infty}f(t)e^{-st}dt
                               \biggr\rvert\\
                             & \leq M\int_0^{\infty}\lvert e^{-st}\rvert dt\\
      \intertext{Now, \(s = \sigma + i\omega\) where
      \(\sigma,\omega\in\mathbb{R}\).
      Then \(\lvert e^{-st}\rvert = e^{t\sigma}\lvert e^{-it\omega}\rvert\)
      since
      \(\lvert e^{-t\sigma}\rvert = \sqrt{e^{-2t\sigma}} = e^{-t\sigma}\).
      Recall the trigonometric identity
      \(e^{i\theta} = \cos(\theta) + i\sin(\theta)\).
      Then \(\lvert e^{-it\omega}\rvert = \sqrt{\Re\{e^{-it\omega}\}^2 +
      \Im\{e^{-it\omega}\}^2} = 1\).}
                             & = M\int_0^{\infty}e^{-t\sigma}dt\eqnumtag
                               \label{ch1sec2prob1a}
    \end{align*}
    \Cref{ch1sec2prob1a} converges when \(e^{-t\sigma}\) is bounded.
    That is, \(-t\sigma < 0\iff t\sigma > 0\iff \sigma > 0\) since
    \(t\in(0,\infty)\) so dividing out by \(t\) doesn't effect the inequality.
    Recall that \(s = \sigma + i\omega\) so
    \(\sigma > 0\Rightarrow\Re\{s\} > 0\) in order for \cref{ch1sec2prob1aLT}
    to converge.
  \item
    Show that \(\mathcal{L}\{f(t)\}(s)\) converges uniformly if
    \(\Re\{s\} > a > 0\).
    \par\smallskip
    Let \(\mathcal{L}\{f(t)\}(s) = F(s)\).
    If the Laplace transform converges uniformly, then for \(\Re\{s\} > b\) and
    for \(b > a\),
    \[
    \sup_{s\geq b}\lvert F_R(s) - F(s)\rvert\to 0
    \]
    as \(R\to\infty\) for each \(b > a\).
    Let \(F_R(s) = \int_0^Rf(t)e^{-st}dt\).
    Suppose \(f(t)\) has exponential order; that is,
    \(\lvert f(t)\rvert = Me^{at}\).
    Then
    \begin{align*}
      \lvert F_R(s) - F(s)\rvert
      & = \biggl\lvert\int_R^{\infty}f(t)e^{-st}dt\biggr\rvert\\
      & \leq \int_R^{\infty}\lvert f(t)\rvert e^{-t\sigma}dt\\
      & \leq M\int_R^{\infty}e^{-t(\sigma - a)}dt\eqnumtag
        \label{ch1sec2prob1b}\\
      & = \frac{M}{\sigma - a}e^{-R(\sigma - a)}
    \end{align*}
    Now for \(\Re\{s\}\geq b > a\),
    \[
    \sup_{\Re\{s\}\geq b}\lvert F_R(s) - F(s)\rvert\leq
    \frac{Me^{-R(b - a)}}{b - a}\to 0
    \]
    as \(R\to\infty\).
    Thus, \(\mathcal{L}\{f(t)\}(s)\) converges uniformly for \(\Re\{s\} > a\).
  \item
    \label{ch1sec2prob1c}
    Show that \(F(s) = \mathcal{L}\{f(t)\}(s)\to 0\) as \(\Re\{s\}\to\infty\).
    \par\smallskip
    From \cref{ch1sec2prob1b}, we have
    \[
    \lvert F(s)\rvert\leq\frac{Me^{-R(\Re\{s\} - a)}}{\Re\{s\} - a}
    \]
    Now \(R\in(0,\infty)\) so \(R > 0\) and \(\Re\{s\} > a > 0\) so
    \(\Re\{s\} - a > 0\).
    \begin{align*}
      \lim_{\Re\{s\}\to\infty}\frac{Me^{-R(\Re\{s\} - a)}}{\Re\{s\} - a}
      & = \frac{M}{e^{\infty}\infty}\\
      & = \frac{M}{\infty}\\
      F(s) & \to 0
    \end{align*}
    as \(\Re\{s\}\to\infty\).
  \end{exercise}
\item
  Let \(f(t) = e^t\) on \([0,\infty)\).
  \begin{exercise}[label = (\alph*), ref = \arabic{exercisei} (\alph*)]
  \item
    Show that \(F(s) = \mathcal{L}\{e^t\}(s)\) converges for \(\Re\{s\} > 1\).
    \begin{align*}
      \biggl\lvert\int_0^{\infty}e^te^{-st}dt\biggr\rvert
      & \leq \int_0^{\infty}e^{-t(\sigma - 1)}dt\\
      & = \frac{-e^{-t(\sigma - 1)}}{\sigma - 1}\biggr|_0^{\infty}
    \end{align*}
    In order for convergence, \(-t(\sigma - 1) < 0\iff\sigma > 1\).
    Since \(s = \sigma + i\omega\), we have that \(F(s)\) converges absolutely
    when \(\sigma = \Re\{s\} > 1\).
  \item
    Show that \(\mathcal{L}\{e^t\}(s)\) converges uniformly if
    \(\Re\{s\} > a > 1\).
    \begin{align*}
      \lvert F_R(s) - F(s)\rvert
      & = \biggl\lvert\int_R^{\infty}e^te^{-st}dt\biggr\rvert\\
      & \leq \int_R^{\infty}e^{-t(\sigma - 1)}dt\\
      & = \frac{e^{-R(\sigma - 1)}}{\sigma - 1}
    \end{align*}
    For \(\Re\{s\}\geq b > 1 > 0\),
    \[
    \sup_{\Re\{s\}\geq b}\lvert F_R(s) - F(s)\rvert\leq
    \frac{e^{-R(b - 1)}}{b - 1}\to 0
    \]
    as \(R\to\infty\) since \(b > 1 > 0\iff b - 1 > 0\iff b > 1\).
    Therefore, \(\mathcal{L}\{e^t\}(s)\) converges uniformly when
    \(\Re\{s\} > 1\).
  \item
    Show that \(F(s) = \mathcal{L}\{e^t\}(s)\to 0\) as \(\Re\{s\}\to\infty\).
    \par\smallskip
    This follows by the same reasoning of \cref{ch1sec2prob1c} with nothing
    new to gain from repeating the process.
  \end{exercise}
\item
  Show that the Laplace transform of the function \(f(t) = 1/t\), \(t > 0\)
  does not exist for any value of \(s\).
  \par\smallskip
  Note the well known gamma function,
  \(\Gamma(t) = \int_0^{\infty}x^{t - 1}e^{-x}dx\).
  Now, the Laplace transform of \(f(t)\) is
  \[
  \mathcal{L}\{1/t\}(s) = \int_0^{\infty}\frac{e^{-st}}{t}dt
  \]
  Let \(st = u\).
  Then \(du = sdt\) and \(1/t = s/u\).
  After making these substitutions, we have
  \[
  \int_0^{\infty}\frac{e^{-st}}{t}dt = s^2\int_0^{\infty}u^{-1}e^{-u}du =
  \Gamma(0)\eqnumtag\label{ch1sec2prob3}
  \]
  By Euler's reflection formula,
  \(\Gamma(z)\Gamma(1 - z) = \frac{\pi}{\sin(z\pi)}\).
  Using Euler's reflection formula and \cref{ch1sec2prob3}, we have that
  \[
  \Gamma(0) = \lim_{z\to 0}\frac{\pi}{\Gamma(1)\sin(z\pi)}
  \]
  For \(n\) a positive integer, \(\Gamma(n) = (n - 1)!\) so \(\Gamma(1) = 1\).
  \[
  \Gamma(0) = \lim_{z\to 0}\frac{\pi}{\sin(z\pi)} = \infty =
  \int_0^{\infty}\frac{e^{-st}}{t}dt = \mathcal{L}\{1/t\}(s)
  \]
  Therefore, the Laplace transform does not converge for \(f(t) = 1/t\).
\end{exercise}

\section{Continuity Requirements}

Discuss the continuity of each of the following functions and locate any jump
discontinuities.
\begin{exercise}
\item
  \(f(t) = \frac{1}{1 + t}\)
  \par\smallskip
  The function \(f(t)\) is continuous for \(t\in\mathbb{R}\setminus\{-1\}\).
  Next, we need to determine what type of discontinuity we have \(t_c = -1\).
  \begin{align*}
    \lim_{t\to -1^-}\frac{1}{1 + t} & = -\infty\\
    \lim_{t\to -1^+}\frac{1}{1 + t} & = \infty
  \end{align*}
  Therefore, \(f(t_c^-)\neq f(t_c^+)\) and neither are finite so we dont have
  jump or removable discontinuity.
\item
  \(g(t) = t\sin(1/t)\) for \(t\neq 0\).
  \par\smallskip
  We need to determine what happens when \(t = 0\).
  Now, sine is bounded by \(\pm 1\); that is, \(-1\leq\sin(1/t)\leq 1\) so
  \(-t\leq t\sin(1/t)\leq t\).
  Since
  \[
  \lim_{t\to 0}-t = \lim_{t\to 0}t = 0,
  \]
  by the squeeze theorem, \(\lim_{t\to 0}t\sin(1/t) = 0\).
  Thus, the left and right limits exists, are finite, and the same so we
  dont have a jump discontinuity at \(t = 0\).
\item
  \(h(t) =
  \begin{cases}
    t, & t\leq 1\\
    \frac{1}{1 + t^2}, & t > 1
  \end{cases}\)
  \par\smallskip
  The only value we need to check is when \(t = 1\) since
  \(t = \pm i\not\in\mathbb{R}\).
  Then \(\lim_{t\to 1^-}h(t) = 1\) and \(\lim_{t\to 1^+}h(t) = 1/2\).
  Therefore, we the left right limits exists, finite, and not equal so we have
  a jump discontinuity at \(t = 1\).
\item
  \(i(t) =
  \begin{cases}
    \frac{\sinh(t)}{t}, & t\neq 0\\
    1, & t = 0
  \end{cases}\)
  \par\smallskip
  This problem is fairly straight forward when we invoke L'H\^{o}pital's rule.
  \[
  \lim_{t\to 0^-}\frac{\sinh(t)}{t} = \frac{0}{0}\Rightarrow
  \lim_{t\to 0^-}\frac{\cosh(t)}{1} = 1 =
  \lim_{t\to 0^+}\frac{\sinh(t)}{t}
  \]
  Additionally, at \(t = 0\), \(i(0) = 1\).
  Therefore, we have no jump discontinuity at \(t = 0\).
\item
  \(j(t) = \frac{1}{t}\sinh(1/t)\) for \(t\neq 0\).
  \par\smallskip
  Recall that the series expansion of
  \(\sinh(t) = \sum_{n = 0}^{\infty}\frac{t^{2n + 1}}{(2n + 1)!}\).
  Then
  \[
  j(t) = \frac{1}{t}\sinh(1/t) =
  \sum_{n = 0}^{\infty}\frac{1}{t^{2n + 2}(2n + 1)!}
  \]
  For \(t\) negative or positive and not equal to zero, \(t^{2n + 2} > 0\).
  Therefore,
  \[
  \lim_{t\to 0}\sum_{n = 0}^{\infty}\frac{1}{t^{2n + 2}(2n + 1)!} = \infty.
  \]
  We do not have a jump discontinuity at \(t = 0\).
\item
  \(k(t) =
  \begin{cases}
    \frac{1 - e^{-t}}{t}, & t\neq 0\\
    0, & t = 0
  \end{cases}\)
  \par\smallskip
  Again, we will invoke L'H\^{o}pital's rule, and in this case,
  \(\lim_{t\to 0}k(t) = 1\).
  At \(t = 0\), \(k(0) = 0\) so we have removable discontinuity at \(t = 0\).
\item
  \(l(t) =
  \begin{cases}
    1, & 2na\leq t < (2n + 1)a\\
    -1, & (2n + 1)a\leq t < (2n + 2)a
  \end{cases}\)
  for \(a > 0\) and \(n = 0,1,\ldots\).
  \par\smallskip
\item
  \(m(t) = \bigl\lfloor\frac{t}{a}\bigr\rfloor\) for \(t\geq 0\), \(a > 0\)
  where \(\lfloor x\rfloor\) is the greatest integer \(\leq x\). 
\end{exercise}

\section{Exponential Order}

%%% Local Variables:
%%% mode: latex
%%% TeX-master: t
%%% End:
